ROOT
@@ -6,5 +6,6 @@ session Learning_Isabelle = HOL +
     Chapter_2_Ex
     Chapter_3
     Chapter_3_Ex
+    Star_Simp_Notes
   document_files
     "root.tex"
